\subsection{Part A}
\[ y^2 = 2 + xy ,\, \frac{dy}{dx} = \frac{y}{2y-x} \]
\[ 2yy' = y(1) + xy' \]
\[ 2yy'- xy' = y  \]
\[ y'(2y- x) = y  \]
\[ y' = \frac{y}{2y-x} \]
\[ \frac{dy}{dx} = \frac{y}{2y-x} \]

\subsection{Part B}
\[ 2yy' = y(1) + xy' \]
\[ y = y + \frac{x}{2} \]
\[ 0 = \frac{x}{2} = x \]
\\
\[ y^2 = 2 + xy \]
\[ y^2 = 2 + (0)y \]
\[ y^2 = 2 \]
\[ y = \pm \sqrt{2} \]
\[ (0, -\sqrt{2}),\,(0, \sqrt{2}) \]

\subsection{Part C}
First constraint:
\[ \frac{dy}{dx} = \frac{y}{2y-x} \]
\[ 0 = \frac{y}{2y-x} \]
$y$ must be zero for the first equation to be fulfilled.
\\
Second constraint:
\[ y^2 = 2 + xy \]
\[ 0^2 \neq 2 + x(0) \]
\[ 0 \neq 2 + x(0) \]
\[ 0 \neq 2 \]
$y$ cannot be zero for the second equation to be fulfilled.

\subsection{Part D}
\[ y^2 = 2 + xy \]
\[ 3^2 = 2 + x(3) \]
\[ 9 = 2 + x(3) \]
\[ 7 = x(3) \]
\[ \frac{7}{3} = x \]
\\
\[ \frac{d}{dt} [y^2 = 2 + xy] \to 2yy' = 0 + x'y + y'x \]
\[ (2)(3)(6) = 3x' + 3x \]
\[ (2)(3)(6) = 3x' + 7 \]
\[ 36 = 3x' + 7 \]
\[ 29 = 3x' \]
\[ \frac{29}{3} = x' \]
\[ \frac{dx}{dt} = \frac{29}{3} \]
