\[ f(0) = 2, \enspace f'(0) = -4, \enspace f''(0) = 3 \]

\subsection{Part A}
\[ g(x) = e^{ax} + f(x) \]
First, we need to know the derivatives of $g(x)$, so we evaluate them as such:
\[ \frac{d}{dx} g(x) = g'(x) = ae^{ax} + f'(x) \]
\[ \frac{d}{dx} g'(x) = g''(x) = e^{ax}a^2 + f''(x) \]
Next, we can evaluate the derivatives of $g(x)$ in line with the pre-defined derivatives of $f(x)$ like so:
\[ g'(0) = ae^{a(0)} + f'(0) = ae^0 - 4 = a - 4 \]
\[ g''(0) = e^{a(0)}a^2 + f''(0) = a^2e^0 + 3 = a^2 + 3 \]
\subsection{Part B}
\[ h(x) = \cos{(kx)}f(x) \]
First, we derive $h(x)$:
\[ \frac{d}{dx} h(x) = h'(x) = -k\sin{(kx)}f(x) + \cos{(kx)}f'(x) \]
This gave us the slope ($h'(0)$), but we still need to find the y value of $h(0)$ and the slope at $h'(0)$
\[ y = h(0) = \cos{[k(0)]}f(0) = \cos{(0)}(2) = (1)(2) = 2 \]
\[ m = h'(0) = -k\sin{(k0)}f(x) + \cos{(k0)}f'(0) = 0 + \cos{(1)}(-4) = -4 \]
We can finally find the tangent equation:
\[ y - 2 = -4 ( x - 0 ) \]
