\subsection{Part A}
\[ y = f(e^2) = \frac{\ln{e^2}}{e^2} = \frac{2}{e^2} \]
\[ m = f'(e^2) = \frac{1 - \ln{e^2}}{(e^2)^2} = \frac{-1}{e^4} \]
\[ y - \frac{2}{e^2} = \frac{-1}{e^4}(x - e^2) \]

\subsection{Part B}
\[ 0 = f'(x) = \frac{1 - \ln{x}}{x^2}, \enspace ln(k) = 1, \enspace k = e, \enspace f'(e) = 0 \]
\[ f''(x) = \frac{(\frac{1}{x})(x^2) - (2x)(1 - \ln{x})}{x^4} \] 
\[ f''(e) = \frac{(\frac{1}{e})(e^2) - (2e)(1 - \ln{e})}{e^4} = \frac{e - 2e + 2e}{e^4} = \frac{e}{e^4} = e^{-3} > 0 \]
$f''(e)$ is positive, so $f(e)$ is just about to increase at this critical point, meaning that this is a local minimum.

\subsection{Part C}
\[ 0 = f''(x) = \frac{x - (2x)(1 - \ln{x})}{x^4} \]
\[ 0 = x - (2x)(1 - \ln{x}), \enspace x = 0\]

\subsection{Part D}
\[ \text{if } \lim_{x \to \infty} \frac{f(x)}{g(x)} = \frac{\infty}{\infty}, \text{ then } \frac{f'(x)}{g'(x)} = \frac{f(x)}{g(x)} \]
\[ \lim_{x \to \infty} f(x) = \lim_{x \to \infty} \frac{\ln{x}}{x}  = \lim_{x \to \infty} \frac{\frac{1}{x}}{1} = \lim_{x \to \infty} \frac{1}{x} = 0 \]
